clean up some proofs.
Also proved a formatting lemma about the output of the traffic manager.

examples/sampler/traffic_manager.v
@@ -1,3 +1,4 @@
+Require Import ProD3.core.PacketFormat.
 Require Import Poulet4.P4light.Syntax.P4defs.
 Require Import Poulet4.P4light.Semantics.Semantics.
 Require Import ProD3.core.Core.
@@ -57,9 +58,30 @@ Definition output_md_to_egress_intr_md (md: OutputMetadata Port) : Val :=
 
 Definition encode_tm_output (elem: EgressPacketDescriptor Port packet) : packet :=
   match elem with
-  | (md, pkt) => PacketFormat.encode (output_md_to_egress_intr_md md) ++ pkt
+  | (md, pkt) => encode (output_md_to_egress_intr_md md) ++ pkt
   end.
+
+Lemma output_is_eg_intr_md:
+  forall md, ⊫ᵥ output_md_to_egress_intr_md md \: egress_intrinsic_metadata_t.
+Proof.
+  intros. destruct md. unfold output_md_to_egress_intr_md. simpl.
+  split; [ repeat constructor | reflexivity].
+Qed.
 
 Definition tofino_tm (ig_intr_tm_md: Sval) (pkt: packet) :=
   qmap encode_tm_output
     (traffic_manager mcast_tbl excl_table (intr_tm_md_to_input_md ig_intr_tm_md, pkt)).
+
+Lemma tofino_tm_output: forall md pkt p,
+    In p (list_rep (tofino_tm md pkt)) ->
+    exists eg_md, ⊫ᵥ eg_md \: egress_intrinsic_metadata_t /\ p ⫢ [⦑ encode eg_md ⦒; ⦑ pkt ⦒].
+Proof.
+  intros. unfold tofino_tm in H. rewrite qmap_map in H. rewrite in_map_iff in H.
+  destruct H as [x [? ?]]. apply traffic_manager_output_snd in H0. simpl in H0.
+  clear md. destruct x as [md out]. simpl in H0. subst out. unfold encode_tm_output in H.
+  exists (output_md_to_egress_intr_md md). split.
+  - apply output_is_eg_intr_md.
+  - subst. exists [encode (output_md_to_egress_intr_md md); pkt]. split.
+    + Opaque encode. simpl. rewrite app_nil_r. Transparent encode. reflexivity.
+    + repeat constructor.
+Qed.
